save point
git-svn-id: https://webdav.seas.upenn.edu/svn/sol/vol@3399 eef5ea85-cc2e-0410-bd84-0fae1f012da8

src/Transforms/dtree.v
@@ -154,22 +154,6 @@ match dt with
 | DT_node l0 _ => l0
 end.
 
-Inductive WF_dtree (f:fdef) : DTree -> Prop :=
-| WDT_node : forall (l0:l) (dts0:DTrees),
-             reachable f l0 ->
-             l0 `notin` dtrees_dom dts0 ->
-             WF_dtrees f l0 dts0 ->
-             WF_dtree f (DT_node l0 dts0)
-with WF_dtrees (f:fdef) : l -> DTrees -> Prop :=
-| WDT_nil : forall l0, WF_dtrees f l0 DT_nil
-| WDT_cons : forall l0 dt0 dts0,
-             imm_domination f l0 (get_dtree_root dt0) ->
-             AtomSetImpl.inter (dtree_dom dt0) (dtrees_dom dts0) [<=] empty ->
-             WF_dtree f dt0 ->
-             WF_dtrees f l0 dts0 ->
-             WF_dtrees f l0 (DT_cons dt0 dts0)
-.
-
 (* l1 >> l2, l1 strict dominates l2 *)
 Definition gt_sdom (res: AMap.t (set l)) (l1 l2:l) : bool :=
 match AMap.get l2 res with
@@ -279,8 +263,8 @@ match chain with
    let b := bound_fdef f in
    let res := dep_doms__nondep_doms b (dom_analyze f) in
    entry `in` dtree_dom dt /\
-   NoDup chain /\ Sorted (gt_sdom_prop res) chain
-| _ => True
+   Sorted (gt_sdom_prop res) chain /\ NoDup chain
+| _ => False
 end.
 
 Definition getEntryLabel (f:fdef) : option l :=
@@ -289,6 +273,15 @@ match f with
 | _ => None
 end.
 
+Lemma compute_sdom_chains__entry: forall f entry rd l0 chain0,
+  getEntryLabel f = Some entry ->
+  reachablity_analysis f =  Some rd ->
+  In (l0, chain0)
+    (compute_sdom_chains
+      (dep_doms__nondep_doms (bound_fdef f) (dom_analyze f)) rd) ->
+  exists chain0', chain0 = entry :: chain0'.
+Admitted.
+
 Lemma compute_sdom_chains__wf_chain: forall f l0 chain0 entry rd,
   getEntryLabel f = Some entry ->
   reachablity_analysis f =  Some rd ->
@@ -296,7 +289,14 @@ Lemma compute_sdom_chains__wf_chain: forall f l0 chain0 entry rd,
     (compute_sdom_chains
        (dep_doms__nondep_doms (bound_fdef f) (dom_analyze f)) rd) ->
   wf_chain f (DT_node entry DT_nil) chain0.
-Admitted.
+Proof.
+  intros.
+  assert (H1':=H1).
+  eapply compute_sdom_chains__entry in H1'; eauto.
+  destruct H1' as [chain0' H1']; subst; simpl.
+  split; auto.
+    eapply compute_sdom_chains_sorted; eauto.
+Qed.
 
 Fixpoint in_children_roots child dts : bool :=
 match dts with
@@ -342,81 +342,12 @@ Definition dtree_mutrec P P' :=
   fun h1 h2 h3 => 
     (pair (@dtree_rec2 P P' h1 h2 h3) (@dtrees_rec2 P P' h1 h2 h3)).
 
-Definition dtree_insert__wf_dtree_prop (dt1:DTree) := 
-forall f p ch dt2,
-  WF_dtree f dt1 ->
-  p `in` dtree_dom dt1 ->
-  imm_domination f p ch ->
-  dtree_insert dt1 p ch = dt2 ->
-  WF_dtree f dt2 /\ is_dtree_edge dt2 p ch /\
-  (is_dtree_edge dt1 p ch -> dt1 = dt2).
-
-Definition dtrees_insert__wf_dtrees_prop (dts1:DTrees) := 
-forall f p ch dts2 root,
-  WF_dtrees f root dts1 ->
-  p `in` dtrees_dom dts1 ->
-  imm_domination f p ch ->
-  dtrees_insert dts1 p ch = dts2 ->
-  WF_dtrees f root dts2 /\ is_dtrees_edge dts2 p ch /\
-  (is_dtrees_edge dts1 p ch -> dts1 = dts2).
-
-Lemma dtree_insert__wf_dtree_mutrec :
-  (forall dt1, dtree_insert__wf_dtree_prop dt1) *
-  (forall dts1, dtrees_insert__wf_dtrees_prop dts1).
-Proof.
-  apply dtree_mutrec; 
-    unfold dtree_insert__wf_dtree_prop, dtrees_insert__wf_dtrees_prop;
-    simpl; intros.
-Admitted.
-
-Lemma dtree_insert__wf_dtree : forall f p ch dt1 dt2,
-  WF_dtree f dt1 ->
-  p `in` dtree_dom dt1 ->
-  imm_domination f p ch ->
-  dtree_insert dt1 p ch = dt2 ->
-  WF_dtree f dt2 /\ is_dtree_edge dt2 p ch /\
-  (is_dtree_edge dt1 p ch -> dt1 = dt2).
-Admitted.
-
 Fixpoint create_dtree_from_chain dt chain : DTree :=
 match chain with
 | p::((ch::_) as chain') => 
     create_dtree_from_chain (dtree_insert dt p ch) chain'
 | _ => dt
 end.
-
-Fixpoint chain_in_dtree chain dt : Prop :=
-match chain with
-| p::((ch::_) as chain') => 
-   is_dtree_edge dt p ch /\ chain_in_dtree chain' dt
-| _ => True
-end.
-
-Lemma create_dtree_from_chain__wf_dtree: forall f dt chain,
-  wf_chain f dt chain ->
-  WF_dtree f dt ->
-  WF_dtree f (create_dtree_from_chain dt chain).
-Admitted.
-
-Lemma create_dtree_from_chain__in_dtree: forall f dt chain,
-  wf_chain f dt chain ->
-  chain_in_dtree chain (create_dtree_from_chain dt chain).
-Admitted.
-
-Lemma create_dtree_from_chain__in_dtree': forall dt chain chain0,
-  chain_in_dtree chain0 dt ->
-  chain_in_dtree chain0 (create_dtree_from_chain dt chain).
-Admitted.
-
-Lemma create_dtree_from_chain__wf_chain: forall f chain0 chain dt,
-  wf_chain f dt chain0 ->
-  wf_chain f (create_dtree_from_chain dt chain) chain0.
-Proof.
-  induction chain; simpl; intros; auto.
-    destruct chain; auto.
-    apply IHchain.    
-
-Admitted.
 
 Definition create_dtree (f: fdef) : option DTree :=
 match getEntryLabel f, reachablity_analysis f with
@@ -430,67 +361,454 @@ match getEntryLabel f, reachablity_analysis f with
 | _, _ => None
 end.
 
-Lemma fold_left_create_dtree_from_chain__wf_dtree: forall f chains dt,
-  (forall l0 chain0, In (l0, chain0) chains -> wf_chain f dt chain0) ->
-  WF_dtree f dt ->
-  WF_dtree f
-    (fold_left
-       (fun (acc : DTree) (elt : l * list id) =>
-        let '(_, chain) := elt in create_dtree_from_chain acc chain) chains 
-       dt).
+Lemma dtrees_insert__in_children_roots: forall ch p0 ch0 dts,
+  in_children_roots ch dts = in_children_roots ch (dtrees_insert dts p0 ch0).
 Proof.
-  induction chains; simpl; intros; auto.
-    destruct a.
-    apply create_dtree_from_chain__wf_dtree with (chain:=l1) in H0; eauto.
-      apply IHchains; auto.
-        intros.
-        apply create_dtree_from_chain__wf_chain; eauto.
+  induction dts; simpl; auto.
+    rewrite <- IHdts.
+    destruct d. simpl.
+    destruct (l_dec l0 ch); subst.
+      destruct (id_dec p0 ch); subst.
+        destruct (in_children_roots ch0 d);
+          destruct (l_dec ch ch); auto; try congruence.
+        destruct (l_dec ch ch); auto; try congruence.
+      destruct (id_dec p0 l0); subst.
+        destruct (in_children_roots ch0 d);
+          destruct (l_dec l0 ch); auto; try congruence.
+        destruct (l_dec l0 ch); auto; try congruence.
 Qed.
 
-Lemma fold_left_create_dtree_from_chain_init_in_dtree: forall chain0 chains dt,
-  chain_in_dtree chain0 dt ->
-  chain_in_dtree chain0
+Definition dtree_insert__is_dtree_edge_prop (dt:DTree) := 
+forall p ch p0 ch0,
+  is_dtree_edge (dtree_insert dt p ch) p0 ch0 <-> 
+  is_dtree_edge dt p0 ch0 \/ (p `in` dtree_dom dt /\ p = p0 /\ ch = ch0).
+
+Fixpoint size_of_dtrees (dts:DTrees) : nat :=
+match dts with
+| DT_nil => O
+| DT_cons _ dts' => S (size_of_dtrees dts')
+end.
+
+Definition dtrees_insert__is_dtrees_edge_prop (dts:DTrees) := 
+forall p ch p0 ch0,
+  is_dtrees_edge (dtrees_insert dts p ch) p0 ch0 <-> 
+  is_dtrees_edge dts p0 ch0 \/ (p `in` dtrees_dom dts /\ p = p0 /\ ch = ch0).
+
+Lemma dtree_insert__is_dtree_edge_mutrec :
+  (forall dt, dtree_insert__is_dtree_edge_prop dt) *
+  (forall dts, dtrees_insert__is_dtrees_edge_prop dts).
+Proof.
+  apply dtree_mutrec; 
+    unfold dtree_insert__is_dtree_edge_prop, dtrees_insert__is_dtrees_edge_prop;
+    simpl; intros.
+
+  Case "1".
+    destruct (id_dec p l0); subst.
+    SCase "1.1".
+      destruct (id_dec p0 l0); subst.
+      SSCase "1.1.1".
+        remember (in_children_roots ch d) as R.
+        destruct R; simpl.
+        SSSCase "1.1.1.1".
+          destruct (id_dec l0 l0); try congruence.
+          split; intro J; auto.
+            destruct J as [J | [J1 [J2 J3]]]; subst; auto.
+            rewrite <- HeqR. reflexivity.
+
+        SSSCase "1.1.1.2".
+          destruct (id_dec l0 l0); try congruence.
+          destruct (l_dec ch ch0); subst.
+          SSSSCase "1.1.1.2.1".
+            split; auto.
+              intros. reflexivity.
+          SSSSCase "1.1.1.2.2".
+            destruct (in_children_roots ch0 d).
+              split; auto.
+                intros. 
+                destruct H0 as [H0 | [J1 J2]]; subst; auto; try congruence.
+              destruct (id_dec l0 ch); subst.
+                split; intros.
+                  apply orb_true_iff in H0.
+                  destruct H0; auto; try congruence.
+
+                  apply orb_true_iff.
+                  destruct H0 as [H0 | [J1 [J2 J3]]]; subst; auto.
+                split; intros.
+                  apply orb_true_iff in H0.
+                  destruct H0; auto; try congruence.
+
+                  apply orb_true_iff.
+                  destruct H0 as [H0 | [J1 [J2 J3]]]; subst; auto.
+      SSCase "1.1.2".
+        remember (in_children_roots ch d) as R.
+        destruct R; simpl.
+        SSSCase "1.1.2.1".
+          destruct (id_dec p0 l0); try congruence.
+          split; intro J; auto.
+            destruct J as [J | [J1 [J2 J3]]]; subst; auto.
+              congruence.
+        SSSCase "1.1.2.2".
+          destruct (id_dec p0 l0); try congruence.
+          destruct (l_dec p0 ch); subst.
+          SSSSCase "1.1.2.2.1".
+            destruct (id_dec ch ch); try congruence.
+            split; intros.
+              apply orb_true_iff in H0.
+              destruct H0; auto; try congruence.
+
+              apply orb_true_iff.
+              destruct H0 as [H0 | [J1 [J2 J3]]]; subst; auto.
+
+          SSSSCase "1.1.2.2.2".
+            destruct (id_dec p0 ch); subst; try congruence.
+            split; intros.
+              apply orb_true_iff in H0.
+              destruct H0; auto; try congruence.
+
+              apply orb_true_iff.
+              destruct H0 as [H0 | [J1 [J2 J3]]]; subst; auto.
+
+    SCase "1.2".
+      simpl.
+      rewrite <- dtrees_insert__in_children_roots.
+      destruct (id_dec p0 l0); subst.
+      SSCase "1.2.1".
+        remember (in_children_roots ch0 d) as R.
+        destruct R; simpl.
+        SSSCase "1.2.1.1".
+          split; intro J; auto.
+            reflexivity.
+        SSSCase "1.2.1.2".
+          split; intro J.
+            apply H in J.
+            destruct J as [J | [J1 [J2 J3]]]; subst; auto.
+
+            apply H.
+            destruct J as [J | [J1 [J2 J3]]]; subst; auto.
+              congruence.
+      SSCase "1.2.2".
+        split; intro J; auto.
+          apply H in J.
+          destruct J as [J | [J1 [J2 J3]]]; subst; auto.
+
+          apply H.
+          destruct J as [J | [J1 [J2 J3]]]; subst; auto.
+            right. fsetdec.
+
+  Case "2".
+    split; intros J.
+       congruence.
+       destruct J as [J | [J1 [J2 J3]]]; subst; auto.
+         fsetdec.
+
+  Case "3".
+    split; intros J.
+      apply orb_true_iff in J.
+      destruct J as [J | J].
+        apply H in J. 
+        destruct J as [J | [J1 [J2 J3]]]; subst.
+          left. apply orb_true_iff. auto.
+          right. fsetdec.
+
+        apply H0 in J. 
+        destruct J as [J | [J1 [J2 J3]]]; subst.
+          left. apply orb_true_iff. auto.
+          right. fsetdec.
+
+      apply orb_true_iff.
+      destruct J as [J | [J1 [J2 J3]]]; subst.
+        apply orb_true_iff in J.
+        destruct J as [J | J].
+          left. apply H; auto.
+          right. apply H0; auto.
+
+        assert (p0 `in` (dtree_dom d) \/ p0 `in` (dtrees_dom d0)) as J.
+          fsetdec.
+        destruct J as [J | J].
+          left. apply H; auto.
+          right. apply H0; auto.
+Qed.
+        
+Lemma dtree_insert__is_dtree_edge : forall p ch p0 ch0 dt ,
+  is_dtree_edge (dtree_insert dt p ch) p0 ch0 <-> 
+  is_dtree_edge dt p0 ch0 \/ (p `in` dtree_dom dt /\ p = p0 /\ ch = ch0).
+Proof.
+  destruct (dtree_insert__is_dtree_edge_mutrec).
+  unfold dtree_insert__is_dtree_edge_prop in *.
+  eauto.
+Qed.
+
+Fixpoint is_chain_edge (chain:list l) p0 ch0 : Prop :=
+match chain with
+| p::((ch::_) as chain') => (p = p0 /\ ch = ch0) \/ is_chain_edge chain' p0 ch0
+| _ => False
+end.
+
+Definition chain_connects_dtree dt (chain:list l) : Prop :=
+match chain with
+| entry :: _ :: _ => entry `in` dtree_dom dt
+| _ => False
+end.
+
+Definition dtree_insert__in_dtree_dom_prop (dt:DTree) := 
+forall p ch,
+  p `in` dtree_dom dt -> is_dtree_edge (dtree_insert dt p ch) p ch.
+
+Definition dtrees_insert__in_dtrees_dom_prop (dts:DTrees) := 
+forall p ch,
+  p `in` dtrees_dom dts ->is_dtrees_edge (dtrees_insert dts p ch) p ch.
+
+Lemma dtree_insert__in_dtree_dom_mutrec :
+  (forall dt, dtree_insert__in_dtree_dom_prop dt) *
+  (forall dts, dtrees_insert__in_dtrees_dom_prop dts).
+Proof.
+  apply dtree_mutrec; 
+    unfold dtree_insert__in_dtree_dom_prop, 
+           dtrees_insert__in_dtrees_dom_prop;
+    simpl; intros.
+
+  destruct (id_dec p l0); subst; simpl.
+    remember (in_children_roots ch d) as R.
+    destruct R; simpl.
+      rewrite <- HeqR.
+      destruct (id_dec l0 l0); try congruence.
+
+      rewrite <- HeqR.
+      destruct (id_dec l0 l0); try congruence.
+      destruct (l_dec ch ch); try congruence.
+
+    destruct (id_dec p l0); subst; try congruence.
+      apply H.
+      assert (p = l0 \/ p `in` dtrees_dom d) as J.
+        clear - H0. fsetdec.
+      destruct J as [J | J]; subst; auto; try congruence.
+
+  contradict H. auto.
+       
+  assert (p `in` (dtree_dom d) \/ p `in` (dtrees_dom d0)) as J.
+    fsetdec.
+  apply orb_true_iff.
+    destruct J as [J | J]. 
+      left. apply H; auto.
+      right. apply H0; auto.
+Qed.
+
+Lemma dtree_insert__in_dtree_dom: forall dt p ch,
+  p `in` dtree_dom dt -> is_dtree_edge (dtree_insert dt p ch) p ch.
+Proof.
+  destruct dtree_insert__in_dtree_dom_mutrec as [H _].
+  unfold dtree_insert__in_dtree_dom_prop in H. auto.
+Qed.
+
+Definition is_dtree_edge__in_dtree_dom_prop (dt:DTree) := 
+forall p ch, is_dtree_edge dt p ch -> 
+  p `in` dtree_dom dt /\ ch `in` dtree_dom dt.
+
+Definition is_dtrees_edge__in_dtrees_dom_prop (dts:DTrees) := 
+forall p ch, is_dtrees_edge dts p ch -> 
+  p `in` dtrees_dom dts /\ ch `in` dtrees_dom dts.
+
+Lemma in_children_roots__dtrees_dom: forall ch dts,
+  in_children_roots ch dts -> ch `in` dtrees_dom dts.
+Proof.
+  induction dts; simpl; intros.
+    congruence.
+
+    destruct d.
+    destruct (l_dec l0 ch); subst; simpl; eauto.
+Qed.
+
+Lemma is_dtree_edge__in_dtree_dom_mutrec :
+  (forall dt, is_dtree_edge__in_dtree_dom_prop dt) *
+  (forall dts, is_dtrees_edge__in_dtrees_dom_prop dts).
+Proof.
+  apply dtree_mutrec; 
+    unfold is_dtree_edge__in_dtree_dom_prop, 
+           is_dtrees_edge__in_dtrees_dom_prop;
+    simpl; intros.
+
+  destruct (id_dec p l0); subst; simpl.
+    remember (in_children_roots ch d) as R.
+    destruct R; simpl.
+      symmetry in HeqR.
+      apply in_children_roots__dtrees_dom in HeqR. fsetdec.
+
+      apply H in H0. destruct H0 as [J1 J2]. auto.
+
+    apply H in H0. destruct H0 as [J1 J2]. auto.
+
+  congruence.
+
+  apply orb_true_iff in H1.
+  destruct H1 as [J | J]. 
+    apply H in J. destruct J; auto.
+    apply H0 in J. destruct J; auto.
+Qed.
+
+Lemma is_dtree_edge__in_dtree_dom: forall dt p ch, 
+  is_dtree_edge dt p ch -> 
+  p `in` dtree_dom dt /\ ch `in` dtree_dom dt.
+Proof.
+  destruct is_dtree_edge__in_dtree_dom_mutrec as [H1 _].
+  unfold is_dtree_edge__in_dtree_dom_prop in H1.
+  auto.
+Qed.
+
+Lemma dtree_insert__ch_in_dtree_dom: forall dt p ch,
+  p `in` dtree_dom dt -> ch `in` dtree_dom (dtree_insert dt p ch).
+Proof.
+  intros.
+  eapply is_dtree_edge__in_dtree_dom.
+  eapply dtree_insert__in_dtree_dom; eauto.
+Qed.
+
+Lemma create_dtree_from_chain__is_dtree_edge__is_chain_edge: 
+  forall p0 ch0 chain dt,
+  (is_dtree_edge (create_dtree_from_chain dt chain) p0 ch0 -> 
+   is_dtree_edge dt p0 ch0 \/is_chain_edge chain p0 ch0) /\
+  (is_dtree_edge dt p0 ch0 \/ 
+   (chain_connects_dtree dt chain /\ is_chain_edge chain p0 ch0) ->
+   is_dtree_edge (create_dtree_from_chain dt chain) p0 ch0).
+Proof.
+  induction chain; simpl; intros.
+    split; intros; tauto.
+     
+    destruct chain.
+      tauto.
+
+      split; intros.
+        apply IHchain in H.
+        destruct H as [H | H]; auto.
+        apply dtree_insert__is_dtree_edge in H.
+        destruct H as [H | [H [H1 H2]]]; subst; auto.
+
+        apply IHchain.
+        destruct H as [H | [H [[H1 H2] | H1]]]; subst.
+          left. apply dtree_insert__is_dtree_edge; auto.
+          left. apply dtree_insert__is_dtree_edge; auto.
+          right. split; auto.
+            destruct chain; simpl in *; auto.
+            apply dtree_insert__ch_in_dtree_dom; auto.
+Qed.
+
+Definition dtree_insert__in_dtree_dom_prop' (dt:DTree) := 
+forall i0 p ch,
+  i0 `in` dtree_dom dt -> i0 `in` dtree_dom (dtree_insert dt p ch).
+
+Definition dtrees_insert__in_dtrees_dom_prop' (dts:DTrees) := 
+forall i0 p ch,
+  i0 `in` dtrees_dom dts -> i0 `in` dtrees_dom (dtrees_insert dts p ch).
+
+Lemma dtree_insert__in_dtree_dom_mutrec' :
+  (forall dt, dtree_insert__in_dtree_dom_prop' dt) *
+  (forall dts, dtrees_insert__in_dtrees_dom_prop' dts).
+Proof.
+  apply dtree_mutrec; 
+    unfold dtree_insert__in_dtree_dom_prop', 
+           dtrees_insert__in_dtrees_dom_prop';
+    simpl; intros.
+
+  destruct (id_dec p l0); subst; simpl.
+    remember (in_children_roots ch d) as R.
+    destruct R; simpl.
+      fsetdec.
+      fsetdec.
+
+    assert (i0 = l0 \/ i0 `in` dtrees_dom d) as J.
+      clear - H0. fsetdec.
+    destruct J as [J | J]; subst; auto; try congruence.
+
+  contradict H. auto.
+       
+  assert (i0 `in` (dtree_dom d) \/ i0 `in` (dtrees_dom d0)) as J.
+    fsetdec.
+  destruct J as [J | J]; eauto.
+Qed.
+
+Lemma dtree_insert__in_dtree_dom': forall dt i0 p ch,
+  i0 `in` dtree_dom dt -> i0 `in` dtree_dom (dtree_insert dt p ch).
+Proof.
+  destruct dtree_insert__in_dtree_dom_mutrec' as [H _].
+  unfold dtree_insert__in_dtree_dom_prop' in H. auto.
+Qed.
+
+Lemma create_dtree_from_chain__chain_connects_dtree: forall chain0 chain dt,
+  chain_connects_dtree dt chain0 ->
+  chain_connects_dtree (create_dtree_from_chain dt chain) chain0.
+Proof.
+  induction chain; simpl; intros; auto.
+    destruct chain; auto.
+    apply IHchain.    
+    destruct chain0; simpl in *; intros; auto.
+    destruct chain0; auto.
+    eapply dtree_insert__in_dtree_dom'; eauto.
+Qed.
+
+Lemma fold_left_create_dtree_from_chain__is_dtree_edge__is_chain_edge: 
+  forall p0 ch0 chains dt,
+  (is_dtree_edge
     (fold_left
       (fun (acc : DTree) (elt : l * list id) =>
        let '(_, chain) := elt in create_dtree_from_chain acc chain)
-     chains dt).
-Proof.
-  induction chains; intros; auto.
-    apply IHchains. destruct a.
-    apply create_dtree_from_chain__in_dtree'; auto.
-Qed.
-
-Lemma fold_left_create_dtree_from_chain__in_dtree: forall f l0 chain0 chains dt,
-  In (l0, chain0) chains -> wf_chain f dt chain0 ->
-  chain_in_dtree chain0
+     chains dt) p0 ch0 -> 
+  (is_dtree_edge dt p0 ch0 \/
+   exists l0, exists chain0, 
+     In (l0, chain0) chains /\ is_chain_edge chain0 p0 ch0)) /\
+  ((is_dtree_edge dt p0 ch0 \/
+   exists l0, exists chain0, 
+     In (l0, chain0) chains /\ chain_connects_dtree dt chain0 /\
+     is_chain_edge chain0 p0 ch0) ->
+   is_dtree_edge
     (fold_left
       (fun (acc : DTree) (elt : l * list id) =>
        let '(_, chain) := elt in create_dtree_from_chain acc chain)
-     chains dt).
+     chains dt) p0 ch0).
 Proof.
   induction chains; simpl; intros.
-    inv H.
+    split; intro J; auto.
+      destruct J as [H | [l0 [chn0 [J1 J2]]]]; auto.
+        inv J1.
 
-    destruct H as [H | H]; subst.
-      apply fold_left_create_dtree_from_chain_init_in_dtree.
-      eapply create_dtree_from_chain__in_dtree; eauto.
+    destruct a.
+    destruct (IHchains (create_dtree_from_chain dt l1)) as [J1 J2].
+    clear IHchains.
+    split; intros J.
+      apply J1 in J.      
+      destruct J as [J | [l2 [chain2 [J3 J4]]]].
+        apply create_dtree_from_chain__is_dtree_edge__is_chain_edge in J.
+        destruct J as [J | J]; auto.
+          right. exists l0. exists l1. auto.
+        right. exists l2. exists chain2. auto.
 
-      apply IHchains; auto.
-      destruct a.
-      apply create_dtree_from_chain__wf_chain; eauto.
+      apply J2.
+      destruct J as [J | [l2 [chain2 [J3 [J4 J5]]]]].
+        left.
+        apply create_dtree_from_chain__is_dtree_edge__is_chain_edge; auto.
+
+        destruct J3 as [J3 | J3].
+          inv J3. left.
+          apply create_dtree_from_chain__is_dtree_edge__is_chain_edge; auto.
+
+          right. exists l2. exists chain2. split; auto. split; auto.
+            apply create_dtree_from_chain__chain_connects_dtree; auto.
 Qed.
 
 Lemma create_dtree__wf_dtree: forall f dt,
   create_dtree f = Some dt ->
-  WF_dtree f dt /\ 
   match getEntryLabel f, reachablity_analysis f with
   | Some root, Some rd =>
       let dt' := dom_analyze f in
       let b := bound_fdef f in
       let chains := compute_sdom_chains (dep_doms__nondep_doms b dt') rd in
-      forall l0 chain0, 
-        In (l0, chain0) chains -> chain_in_dtree chain0 dt
-  | _, _ => True
+      forall p0 ch0,
+        (is_dtree_edge dt p0 ch0 -> 
+         exists l0, exists chain0, 
+           In (l0, chain0) chains /\ is_chain_edge chain0 p0 ch0) /\
+        ((exists l0, exists chain0, 
+           In (l0, chain0) chains /\ 
+           chain_connects_dtree (DT_node root DT_nil) chain0 /\
+           is_chain_edge chain0 p0 ch0) -> is_dtree_edge dt p0 ch0)
+  | _, _ => False
   end.
 Proof.
   unfold create_dtree.
@@ -499,15 +817,15 @@ Proof.
   destruct R; tinv H.
   remember (reachablity_analysis f) as R.
   destruct R; inv H.
-  split. 
-    apply fold_left_create_dtree_from_chain__wf_dtree.
-      intros. eapply compute_sdom_chains__wf_chain; eauto.
-      apply WDT_node; auto.
-        admit. (*reach*)
-        constructor.
-    intros.
-    eapply fold_left_create_dtree_from_chain__in_dtree; eauto.
-      eapply compute_sdom_chains__wf_chain; eauto.    
+  intros.
+  destruct (@fold_left_create_dtree_from_chain__is_dtree_edge__is_chain_edge
+    p0 ch0 (compute_sdom_chains
+             (dep_doms__nondep_doms (bound_fdef f) (dom_analyze f)) l1)
+    (DT_node l0 DT_nil)) as [J1 J2].
+  split; intros J; auto.
+    apply J1 in J.
+    destruct J as [J | J]; auto.
+      simpl in J. destruct (id_dec p0 l0); tinv J.
 Qed.
 
 Fixpoint find_idom_aux (res: AMap.t (set l)) (acc:l) (dts: set l): option l :=
@@ -545,1128 +863,6 @@ match bd with
     | Some l1 => compute_idoms res bd' ((l1,l0)::acc)
     end
 end.
-
-(*
-Require Import Orders.
-
-Module NatOrder <: TotalLeBool.
-
-Section A.
- 
-  Variable f: fdef.
-  Variable l0: l.
-  Hypothesis Hreach: reachable f l0.
-
-  Definition t := {l0: l & }.
-  Fixpoint leb x y :=
-    match x, y with
-    | O, _ => true
-    | _, O => false
-    | S x', S y' => leb x' y'
-    end.
-  Infix "<=?" := leb (at level 35).
-  Theorem leb_total : forall a1 a2, a1 <=? a2 \/ a2 <=? a1. admit. Qed.
-
-End A.
-
-End NatOrder.
-
-Lemma sdom_ordered : forall f l1 l2 l3
-  (Hneq: l1 <> l2) (Hreach: reachable f l3)
-  (Hsdom: strict_domination f l1 l3)
-  (Hsdom': strict_domination f l2 l3),
-  strict_domination f l1 l2 \/ strict_domination f l2 l1.
-Proof.
-  intros.
-  apply sdom_sdom' in Hsdom; auto.
-  apply sdom_sdom' in Hsdom'; auto.
-  assert (J:=Hsdom').
-  eapply sdom_ordered' in J; eauto.
-  destruct J as [[J1 J2] | [J1 J2]].
-    left. apply dom_sdom; auto.
-    right. apply dom_sdom; auto.
-Qed.
-
-Require Import Sorting.
-
-Module Import NatSort := Sort NatOrder.
-
-Check sort.
-
-Eval compute in sort (5::3::6::1::8::6::0::nil)%nat.
-*)
-
-(*
-Fixpoint find_idom_aux (res: AMap.t (set l)) (acc:l) (dts: set l): option l :=
-match dts with
-| nil => Some acc
-| l0::dts' =>
-    match AMap.get l0 res, AMap.get acc res with
-    | dts1, dts2 =>
-        if (in_dec l_dec l0 dts2)
-        then (* acc << l0 *)
-          find_idom_aux res acc dts' 
-        else
-          if (in_dec l_dec acc dts1)
-          then (* l0 << acc *)
-            find_idom_aux res l0 dts' 
-          else (* l0 and acc are incompariable *)
-            None
-    end
-end.
-
-(* We should prove that this function is not partial. *)
-Definition find_idom (res: AMap.t (set l)) (l0:l) : option l :=
-match AMap.get l0 res with
-| l1::dts0 => find_idom_aux res l1 dts0
-| _ => None
-end.
-
-(*
-Fixpoint tree2dtree vs es (tree: Tree vs es) : option DTree :=
-match tree with
-| T_root (index le) => Some (DT_node le DT_nil)
-| T_leaf vs' es' t' (index child) (index parent) _ _ => 
-    match tree2dtree vs' es' t' with
-    | Some dt' => dtree_insert dt' parent child
-    | _ => None
-    end
-| T_eq vs1 vs2 es1 es2 _ _ t1 => tree2dtree vs1 es1 t1
-end.
-*)
-
-Definition PreDTree := list (l * list l).
-
-Definition getEntryLabel (f:fdef) : option l :=
-match f with
-| fdef_intro _ ((block_intro l0 _ _ _)::_) => Some l0
-| _ => None
-end.
-
-Fixpoint cdom (pdt: PreDTree) : atoms :=
-match pdt with
-| nil => empty
-| (_, children)::pdt' => 
-    fold_left (fun acc child => add child acc) children (cdom pdt') 
-end.
-
-Inductive WF_idoms f : list (l*l) -> Prop :=
-| WF_idoms_nil : WF_idoms f nil 
-| WF_idoms_cons : forall l1 l2 idoms, 
-    imm_domination f l1 l2 -> WF_idoms f idoms ->
-    WF_idoms f ((l1,l2)::idoms)
-.
-
-Inductive WF_predtree (f:fdef) : PreDTree -> Prop :=
-| WPDT_entry : forall entry children,
-    getEntryLabel f = Some entry ->
-    (forall child, In child children -> imm_domination f entry child) ->
-    NoDup children ->
-    WF_predtree f ((entry, children)::nil)
-| WPDT_cons : forall parent children pdt,
-    WF_predtree f pdt ->
-    reachable f parent ->
-    (forall child, In child children -> 
-       imm_domination f parent child /\ child `notin` dom pdt `union` cdom pdt) ->
-    NoDup children ->
-    parent `notin` dom pdt ->
-    (exists ancestor, exists parents,
-      In (ancestor, parents) pdt /\ In parent parents) -> 
-    WF_predtree f ((parent, children) :: pdt).
-
-Fixpoint dtree_insert dt parent children : option DTree :=
-match dt with
-| DT_node l0 dts0 => 
-    if (id_dec parent l0) then 
-      Some (DT_node l0 
-        (fold_left (fun acc child => DT_cons (DT_node child DT_nil) acc) 
-          children dts0))
-    else 
-      match dtrees_insert dts0 parent children with
-      | Some dts1 => Some (DT_node l0 dts1)
-      | None => None
-      end
-end
-with dtrees_insert (dts: DTrees) parent children : option DTrees :=
-match dts with
-| DT_nil => Some DT_nil
-| DT_cons dt0 dts0 => 
-    match dtree_insert dt0 parent children, 
-          dtrees_insert dts0 parent children with
-    | Some dt1, Some dts1 => Some (DT_cons dt1 dts1)
-    | _, _ => None
-    end
-end.
-
-Fixpoint predtree2dtree (pdt: PreDTree) : option DTree :=
-match pdt with
-| nil => None
-| (p, chs) :: nil =>
-    Some (DT_node p
-      (fold_left (fun acc child => DT_cons (DT_node child DT_nil) acc) 
-         chs DT_nil))
-| (p, chs) :: pdt' =>
-    match predtree2dtree pdt' with
-    | Some dt' => dtree_insert dt' p chs
-    | _ => None
-    end
-end.
-
-Lemma wf_predtree__wf_dtree__helper: forall f p chs dts0
-  (H0 : reachable f p)
-  (H1 : forall child : l, In child chs -> 
-        imm_domination f p child /\ child `notin` dtrees_dom dts0)
-  (h2 : NoDup chs),
-  WF_dtrees f p dts0 ->
-  WF_dtrees f p
-       (fold_left
-          (fun (acc : DTrees) (child : l) =>
-           DT_cons (DT_node child DT_nil) acc) chs dts0).
-Proof.
-  induction chs; simpl; intros; auto.
-    inv h2.
-    apply IHchs; auto.
-      intros.
-      assert (a = child \/ In child chs) as Hin. auto.
-      apply H1 in Hin.
-      destruct Hin as [J1 J2].
-      simpl. split; auto.
-      assert (child <> a) as Hneq.
-        destruct (l_dec child a); subst; auto.
-          fsetdec.
-
-      assert (a = a \/ In a chs) as Hin. auto.
-      apply H1 in Hin.
-      destruct Hin as [J1 J2].
-      apply WDT_cons; simpl; auto.
-        fsetdec.
-        apply WDT_node; auto.
-          admit.
-          apply WDT_nil.
-Qed.
-
-Scheme dtree_rec2 := Induction for DTree Sort Set
-  with dtrees_rec2 := Induction for DTrees Sort Set.
-
-Definition dtree_mutrec P P' :=
-  fun h1 h2 h3 => 
-    (pair (@dtree_rec2 P P' h1 h2 h3) (@dtrees_rec2 P P' h1 h2 h3)).
-
-Definition dtree_insert__wf_dtree_prop (dt1:DTree) := 
-forall f a1 a0,
-  WF_dtree f dt1 ->
-  exists dt2, dtree_insert dt1 a1 a0 = ret dt2 /\ WF_dtree f dt2.
-
-Definition dtrees_insert__wf_dtrees_prop (dts1:DTrees) := 
-forall f root a1 a0,
-  WF_dtrees f root dts1 ->
-  exists dts2, dtrees_insert dts1 a1 a0 = ret dts2 /\ WF_dtrees f root dts2.
-
-Lemma dtree_insert__wf_dtree_mutrec :
-  (forall dt1, dtree_insert__wf_dtree_prop dt1) *
-  (forall dts1, dtrees_insert__wf_dtrees_prop dts1).
-Proof.
-  apply dtree_mutrec; 
-    unfold dtree_insert__wf_dtree_prop, dtrees_insert__wf_dtrees_prop;
-    simpl; intros.
-Admitted.
-
-Lemma dtree_insert__wf_dtree: forall f dt1 a1 a0,
-  WF_dtree f dt1 ->
-  exists dt2, dtree_insert dt1 a1 a0 = ret dt2 /\ WF_dtree f dt2.
-Proof.
-  destruct dtree_insert__wf_dtree_mutrec as [J1 _].
-  unfold dtree_insert__wf_dtree_prop in J1. auto.
-Qed.
-
-Lemma WF_idoms_elim: forall f p ch idoms,
-  WF_idoms f idoms -> In (p, ch) idoms -> imm_domination f p ch.
-Admitted.
-
-Lemma wf_predtree__wf_dtree : forall f pdts,
-  WF_predtree f pdts ->
-  exists dt, predtree2dtree pdts = Some dt /\ WF_dtree f dt.
-Proof.
-  intros.
-  induction H; simpl.
-    exists 
-      (DT_node entry
-         (fold_left
-            (fun (acc : DTrees) (child : l) =>
-             DT_cons (DT_node child DT_nil) acc) children DT_nil)).
-    split; auto.
-      apply WDT_node.
-        admit.
-        admit.
-        apply wf_predtree__wf_dtree__helper; auto.
-          admit. 
-          apply WDT_nil.
-
-    destruct pdt; tinv H.
-    destruct IHWF_predtree as [dt [J1 J2]].
-    rewrite J1.
-    apply dtree_insert__wf_dtree; auto.
-Qed.
-
-Fixpoint find_children (res: AMap.t (set l)) (root:l) 
-  (others:set l) (acc:list l): option (list l) :=
-match others with 
-| nil => Some acc
-| l0::others' =>
-    match find_idom res l0 with
-    | None => None
-    | Some l1 =>
-        if (id_dec root l1) then
-          if (in_dec l_dec l0 acc) 
-          then find_children res root others' acc
-          else find_children res root others' (l0::acc) 
-        else find_children res root others' acc        
-    end
-end.
-
-Lemma find_children_spec1_aux: forall res root others l0 acc children, 
-  find_children res root others acc = ret children ->
-  In l0 children ->
-  In l0 others \/ In l0 acc.
-Proof.
-  induction others; simpl; intros.
-    inv H; auto.
-
-    destruct (find_idom res a); tinv H.
-    destruct (id_dec root l1); subst.
-      destruct (in_dec l_dec a acc).
-        eapply IHothers in H; eauto.
-          destruct H; auto.
-        eapply IHothers in H; eauto.
-          destruct H; auto.
-          simpl in H. destruct H; subst; auto.
-      eapply IHothers in H; eauto.
-      destruct H; auto.
-Qed.
-
-Lemma find_children_spec1: forall res root others children, 
-  find_children res root others nil = ret children ->
-  incl children others.
-Proof.
-  intros. intros x Jx.
-  eapply find_children_spec1_aux in H; eauto.
-  destruct H; auto. inv H.
-Qed.
-
-Lemma find_children_spec2_aux: forall res root others acc children, 
-  NoDup acc ->
-  find_children res root others acc = ret children ->
-  NoDup children.
-Proof.
-  induction others; simpl; intros.
-    inv H0; auto.
-
-    destruct (find_idom res a); tinv H0.
-    destruct (id_dec root l0); subst; eauto.
-    destruct (in_dec l_dec a acc); eauto.
-Qed.
-
-Lemma find_children_spec2: forall res root others children, 
-  find_children res root others nil = ret children ->
-  NoDup children.
-Proof.
-  intros.
-  eapply find_children_spec2_aux in H; eauto.
-Qed.
-
-Lemma fold_left_remove_in_length_aux: forall (children others' others:list atom),
-  NoDup children ->
-  incl children others' ->
-  incl others' others ->
-  (length others' <= length others)%nat ->
-  children <> nil ->
-  (length (fold_left
-    (fun (acc0 : list atom) (l0 : id) => List.remove eq_atom_dec l0 acc0)
-      children others') < length others)%nat.
-Proof.
-  induction children; simpl; intros.
-    congruence.
-
-    assert (In a others') as Hin.
-      apply H0; simpl; auto.
-    assert (J:=@remove_in_length _ eq_atom_dec a others' Hin).
-    assert ((length (List.remove eq_atom_dec a others') < length others)%nat) 
-      as J'.
-      omega.
-    inv H.
-    destruct children.
-      simpl. auto.
-
-      apply IHchildren; auto.
-        intros x Jx.
-        assert (In x (a :: a0 :: children)) as Hin'.
-          simpl in Jx. destruct Jx; subst; simpl; auto.
-        apply H0 in Hin'.
-        apply remove_neq_in; auto.
-        destruct (id_dec x a); subst; auto.
-
-        intros x Jx. 
-        apply H1.
-        apply remove_neq_in' in Jx; auto.
-        destruct Jx as [Jx1 Jx2]; auto.
-        omega.
-
-        intro J0. inv J0.
-Qed.
-
-Lemma fold_left_remove_in_length: forall (children others:list atom),
-  NoDup children ->
-  incl children others ->
-  children <> nil ->
-  (length (fold_left
-    (fun (acc0 : list atom) (l0 : id) => List.remove eq_atom_dec l0 acc0)
-      children others) < length others)%nat.
-Proof.
-  intros.
-  apply fold_left_remove_in_length_aux; auto.
-    apply incl_refl.
-Qed.
-
-Fixpoint find_next_children (idoms: list (l * l)) (parent: l) (acc : list l)
-  (others: set l) : list l * set l :=
-match idoms with
-| nil => (acc, others)
-| (l1, l2)::idoms' =>
-    if (l_dec l1 parent) then 
-      if (in_dec l_dec l2 others) then
-        find_next_children idoms' parent (l2::acc) (List.remove l_dec l2 others)
-      else find_next_children idoms' parent acc others
-    else find_next_children idoms' parent acc others
-end.
-
-Fixpoint find_next_children_from_children (idoms: list (l * l)) (children:list l)
-  (others: set l) : option (l * list l * set l) :=
-match children with
-| nil => None
-| ch::children' =>
-    match find_next_children idoms ch nil others with
-    | (nil, _) => find_next_children_from_children idoms children' others
-    | (children0, others') => Some (ch, children0, others')
-    end
-end.
-
-Fixpoint find_next_sub_predtree_aux (idoms: list (l * l)) (pdt0 pdt:PreDTree) 
-  (others:set l) : option (PreDTree * set l) :=
-match pdt with
-| nil => None
-| (p, chs)::pdt' => 
-    match find_next_children_from_children idoms chs others with
-    | None => find_next_sub_predtree_aux idoms pdt0 pdt' others
-    | Some (ch, chs', others') => Some ((ch, chs')::pdt0, others')
-    end
-end.
-
-Definition find_next_sub_predtree (idoms: list (l * l)) (pdt:PreDTree) 
-  (others:set l) : option (PreDTree * set l) :=
-find_next_sub_predtree_aux idoms pdt pdt others.
-
-Lemma in_singleton_inv: forall A (a b:A), In a [b] -> a = b.
-Proof.
-  intros.
-  simpl in H. destruct H; auto. inv H.
-Qed.
-
-Lemma find_next_children_inv : forall p idoms chs others chs' others',
-  find_next_children idoms p chs others = (chs', others') ->
-  exists chs'', chs' = chs'' ++ chs /\
-    others' = fold_right (fun ch acc => List.remove l_dec ch acc) others chs'' /\
-    (forall ch, In ch chs'' -> In ch others /\ In (p, ch) idoms).
-Proof.
-  induction idoms; simpl; intros.
-    inv H.
-    exists nil. simpl.
-    split; auto.
-    split; auto. 
-      intros. inversion H.
-
-    destruct a.
-    destruct (l_dec l0 p); subst.
-      destruct (in_dec l_dec l1 others).
-        apply IHidoms in H.
-        destruct H as [chs'' [J1 [J2 J3]]]; subst.
-        exists (chs''++[l1]).
-        simpl_env.
-        split; auto.
-        split.
-          rewrite fold_right_app. simpl. auto.
-
-          intros ch Hin.
-          apply in_app_or in Hin.
-          destruct Hin as [Hin | Hin].
-            apply J3 in Hin.
-            destruct Hin as [J2 J4].
-            split; auto.
-              apply remove_neq_in' in J2.
-              destruct J2; auto.
-
-            apply in_singleton_inv in Hin; subst.
-            split; auto.
-    
-        apply IHidoms in H.
-        destruct H as [chs'' [J1 [J2 J3]]]; subst.
-        exists chs''.
-        split; auto.
-        split; auto.
-          intros ch Hin.
-          apply J3 in Hin.
-          destruct Hin as [J2 J4].
-          split; auto.
-      apply IHidoms in H.
-      destruct H as [chs'' [J1 [J2 J3]]]; subst.
-      exists chs''.
-      split; auto.
-      split; auto.
-        intros ch Hin.
-        apply J3 in Hin.
-        destruct Hin as [J2 J4].
-        split; auto.
-Qed.       
-
-Lemma find_next_children_from_children_inv: forall idoms chs others ch chs' others',
-  find_next_children_from_children idoms chs others = ret (ch, chs', others') ->
-  others' = fold_right (fun ch0 acc => List.remove l_dec ch0 acc) others chs' /\
-  In ch chs /\ (forall ch', In ch' chs' -> In ch' others /\ In (ch, ch') idoms)
-  /\ chs' <> nil.
-Proof.
-  induction chs; simpl; intros.
-    inv H.
-
-    remember (find_next_children idoms a nil others) as R.
-    destruct R.
-    destruct l0; auto.
-      apply IHchs in H.
-      destruct H as [J1 [J2 J3]].
-      split; auto.
-
-      inv H.
-      symmetry in HeqR.
-      apply find_next_children_inv in HeqR; auto.
-      destruct HeqR as [chs'' [J1 [J2 J3]]]; subst.
-      simpl_env in J1. subst.
-      split; auto.
-      split; auto.
-      split; auto.
-        intro J. inv J.
-Qed.
-
-Lemma find_next_sub_predtree_aux_inv: forall idoms pdt0 pdt others pdt' 
-  others',
-  find_next_sub_predtree_aux idoms pdt0 pdt others = Some (pdt', others') ->
-  exists p, exists chs, 
-    pdt' = (p,chs)::pdt0 /\ 
-    others' = fold_right (fun ch0 acc => List.remove l_dec ch0 acc) others chs /\
-    (forall ch, In ch chs -> In ch others /\ In (p, ch) idoms) /\ chs <> nil /\
-    exists p', exists chs', In (p', chs') pdt /\ In p chs'.
-Proof.
-  induction pdt; simpl; intros.
-    inv H.
-
-    destruct a.
-    remember (find_next_children_from_children idoms l1 others) as R.
-    destruct R as [[[ch ch'] others'']|].
-      inv H.
-      exists ch. exists ch'. 
-      symmetry in HeqR.
-      apply find_next_children_from_children_inv in HeqR.
-      destruct HeqR as [J1 [J2 [J3 J4]]]; subst.
-      split; auto.
-      split; auto.
-      split; auto.
-      split; auto.
-        exists l0. exists l1. split; auto.
-
-      apply IHpdt in H; auto.
-      destruct H as [p [chs [Heq1 [Heq2 [J1 [J0 [p' [chs' [J2 J3]]]]]]]]]; 
-        subst.
-      exists p. exists chs. 
-      split; auto.
-      split; auto.
-      split; auto.
-      split; auto.
-        exists p'. exists chs'. split; auto.
-Qed.
-
-Lemma find_next_sub_predtree_inv: forall idoms pdt others pdt' 
-  others',
-  find_next_sub_predtree idoms pdt others = Some (pdt', others') ->
-  exists p, exists chs, 
-    pdt' = (p,chs)::pdt /\ 
-    others' = fold_right (fun ch0 acc => List.remove l_dec ch0 acc) others chs /\
-    (forall ch, In ch chs -> In ch others /\ In (p, ch) idoms) /\ chs <> nil /\
-    exists p', exists chs', In (p', chs') pdt /\ In p chs'.
-Proof.
-  intros. unfold find_next_sub_predtree in H.
-  apply find_next_sub_predtree_aux_inv in H; auto.
-Qed.
-
-Lemma fold_right_remove_length: forall chs others
-  (J1 : forall ch : l, In ch chs -> In ch others)
-  (J0 : chs <> nil),
-  (length
-     (fold_right
-        (fun (ch0 : l) (acc0 : list l) => List.remove l_dec ch0 acc0) others
-        chs) < length others)%nat.
-Proof.
-  induction chs; simpl; intros.
-    congruence.
-
-    destruct chs.
-      simpl.
-      apply remove_in_length; auto.
-
-      assert (length
-               (fold_right
-                  (fun (ch0 : l) (acc0 : list l) => List.remove l_dec ch0 acc0)
-                  others (l0::chs)) < length others)%nat as J.
-        apply IHchs; auto.
-          intro J. inv J.
-      assert (G:=@remove_length _ l_dec a (fold_right
-                  (fun (ch0 : l) (acc0 : list l) => List.remove l_dec ch0 acc0)
-                  others (l0::chs))).
-      omega.
-Qed.
-
-Lemma find_next_sub_predtree_length: forall idoms acc others acc' others',
-  find_next_sub_predtree idoms acc others = ret (acc', others') ->
-  (length others' < length others)%nat.
-Proof.
-  intros.
-  apply find_next_sub_predtree_inv in H.
-  destruct H as [p [chs [Heq1 [Heq2 [J1 [J0 [p' [chs' [J2 J3]]]]]]]]]; subst.
-  apply fold_right_remove_length; auto.
-  intros ch Hin. apply J1 in Hin. destruct Hin; auto.
-Qed.
-
-Program Fixpoint create_predtree_aux (others:set l) (idoms: list (l * l)) 
-  (acc:PreDTree) {measure (List.length others)} : option PreDTree :=
-match others with
-| nil => Some acc
-| _ =>
-   match find_next_sub_predtree idoms acc others with
-   | None => None
-   | Some (acc', others') => create_predtree_aux others' idoms acc'
-   end
-end.
-Next Obligation. 
-  eapply find_next_sub_predtree_length; eauto.
-Qed.
-
-Fixpoint init_predtree (idoms: list (l * l)) (root:l) (others:set l)
-  : option (PreDTree * list l) :=
-match find_next_children idoms root nil others with
-| (nil, _) => None
-| (children, others') => Some ([(root, children)], others')
-end.
-
-Definition create_dtree (f: fdef) : option DTree :=
-match getEntryBlock f, reachablity_analysis f with
-| Some (block_intro root _ _ _), Some rd =>
-    let dt := dom_analyze f in
-    let b := bound_fdef f in
-    let idoms := compute_idoms (dep_doms__nondep_doms b dt) rd nil in
-    match init_predtree idoms root (List.remove eq_atom_dec root rd) with
-    | None => None
-    | Some (pdt0, others) =>
-        match (create_predtree_aux others idoms pdt0) with
-        | None => None
-        | Some pdt => predtree2dtree pdt
-        end
-    end
-| _, _ => None
-end.
-
-Lemma in_predtree_dom: forall p chs (pdt0:PreDTree),
-  In (p, chs) pdt0 -> p `in` dom pdt0.
-Proof.
-  induction pdt0; simpl; intros.
-    inv H.
-    destruct H as [H | H]; subst.
-      fsetdec.
-
-      destruct a.
-      apply IHpdt0 in H.
-      fsetdec.
-Qed.
-
-Lemma in_fold_left_atoms: forall ch chs init
-  (H0 : In ch chs \/ ch `in` init),
-  ch `in` fold_left (fun (acc : atoms) (child : atom) => add child acc) chs init.
-Proof.
-  induction chs; simpl; intros.
-    destruct H0; auto.
-      inv H.
-    destruct H0 as [[H0 | H0] | H0]; subst; eauto.
-Qed.
-
-Lemma in_predtree_cdom: forall p chs ch pdt0,
-  In (p, chs) pdt0 -> In ch chs -> ch `in` cdom pdt0.
-Proof.
-  induction pdt0; simpl; intros.
-    inv H.
-    destruct H as [H | H]; subst.
-      apply in_fold_left_atoms; auto.
-    destruct a.
-    apply in_fold_left_atoms; auto.
-Qed.
-
-Definition P_create_predtree_aux__WF_predtree (n:nat) :=
-  forall f idoms (Hwfi: WF_idoms f idoms) pdt0 others pdt
-  (Hdis: forall l0, 
-    In l0 others -> 
-    l0 `notin` dom pdt0 `union` cdom pdt0),
-  List.length others = n ->
-  WF_predtree f pdt0 ->
-  create_predtree_aux others idoms pdt0 = Some pdt ->
-  WF_predtree f pdt.
-
-Require Import Program.
-
-Ltac simple_create_predtree_aux :=
-  unfold create_predtree_aux, create_predtree_aux_func;
-  rewrite WfExtensionality.fix_sub_eq_ext;
-  repeat fold_sub create_predtree_aux_func ; simpl proj1_sig;
-  simpl. 
-
-Lemma in_fold_right_remove: forall p chs others
-  (Hin : In p
-          (fold_right
-             (fun (ch0 : l) (acc : list l) => List.remove l_dec ch0 acc)
-             others chs)),
-  In p others /\ ~ In p chs.
-Proof.
-  induction chs; simpl; intros.
-    split; auto.
-
-    apply remove_neq_in' in Hin; auto.
-    destruct Hin as [J1 J2].
-    apply IHchs in J1.
-    destruct J1 as [J1 J3].
-    split; auto.
-      intro J. destruct J as [J | J]; auto.
-Qed.
-
-Lemma notin_fold_left_atoms: forall ch chs init,
-  ~ In ch chs -> ch `notin` init -> 
-  ch `notin` 
-    fold_left (fun (acc : atoms) (child : atom) => add child acc) chs init.
-Proof.
-  induction chs; simpl; intros; auto.
-Qed.
-
-Lemma find_next_sub_predtree_fresh: forall (pdt0 : list (atom * list l)) idoms
-  (others : list atom) (pdt : PreDTree)
-  (Hdis : forall l0 : atom,
-          In l0 others -> l0 `notin` union (dom pdt0) (cdom pdt0))
-  (acc' : PreDTree) (others' : set l)
-  (HeqR : ret (acc', others') =
-          find_next_sub_predtree idoms pdt0 others),
-  forall l0 : atom, In l0 others' -> l0 `notin` union (dom acc') (cdom acc').
-Proof.
-  intros.
-  symmetry in HeqR.
-  apply find_next_sub_predtree_inv in HeqR.
-  destruct HeqR as [p [chs [Heq [J1 [J2 [J3 [p' [chs' [J4 J5]]]]]]]]]; subst.
-  simpl.
-  apply in_fold_right_remove in H.
-  destruct H as [J6 J7].
-  apply Hdis in J6.
-  assert (l0 `notin` 
-       (fold_left (fun (acc : atoms) (child : atom) => add child acc)
-          chs (cdom pdt0))) as J8.
-    apply notin_fold_left_atoms; auto.
-  assert (l0 <> p) as Hneq.
-    destruct (l_dec l0 p); subst; auto.
-    eapply in_predtree_cdom in J4; eauto.
-  fsetdec.
-Qed.
-
-Lemma WF_predtree__reachable: forall f pdt p chs ch,
-  WF_predtree f pdt ->
-  In (p, chs) pdt ->
-  In ch chs ->
-  reachable f ch.
-Admitted.
-
-Lemma find_next_sub_predtree_wf_predtree: 
-  forall f idoms (Hwfi: WF_idoms f idoms) pdt (Hwf:WF_predtree f pdt) 
-    others pdt' others'
-  (Hdis: forall l0, 
-    In l0 others -> 
-    l0 `notin` dom pdt `union` cdom pdt),
-  find_next_sub_predtree idoms pdt others = ret (pdt', others') ->
-  WF_predtree f pdt'.
-Proof.
-  intros.
-  apply find_next_sub_predtree_inv in H.
-  destruct H as [p [chs [Heq [J1 [J2 [J3 [p' [chs' [J4 J5]]]]]]]]]; subst.
-  apply WPDT_cons; auto.
-    eapply WF_predtree__reachable in J4; eauto.
-
-    intros child Hin.
-    apply J2 in Hin.
-    destruct Hin as [Hin1 Hin2].
-    split; auto.
-      eapply WF_idoms_elim; eauto.
-
-    admit.
-
-    
-
-Lemma find_next_sub_predtree_aux_wf_predtree: 
-  forall f idoms (Hwfi: WF_idoms f idoms) acc prefix 
-    (Hwf:WF_predtree f (prefix++acc)) others acc' others'
-  (Hdis: forall l0, 
-    In l0 others -> 
-    l0 `notin` dom (prefix++acc) `union` cdom (prefix++acc)),
-  find_next_sub_predtree_aux idoms (prefix++acc) acc others = 
-    ret (acc', others') ->
-  WF_predtree f acc'.
-Proof.
-  intros.
-  applu 
-
-
-  induction acc; simpl; intros.
-    congruence.
-
-    destruct a.
-    remember (find_next_child idoms l1 others) as R.
-    destruct R.
-      inv H.
-      apply WPDT_cons; auto.
-        apply WF_predtree__reachable with (l1:=l0)(l2:=l1) in Hwf.
-          destruct Hwf; auto.
-          apply in_middle.
-        eapply find_next_child__imm_domination; eauto.
-
-        symmetry in HeqR.
-        apply find_next_child_inv in HeqR.
-        destruct HeqR as [J1 J2]. auto.
-
-        right.
-        exists l0. apply in_middle.
-
-      remember (find_next_child idoms l0 others) as R.
-      destruct R.
-        inv H.
-        apply WPDT_cons; auto.
-          apply WF_predtree__reachable with (l1:=l0)(l2:=l1) in Hwf.
-            destruct Hwf; auto.
-            apply in_middle.
-          eapply find_next_child__imm_domination; eauto.
-
-          symmetry in HeqR0.
-          apply find_next_child_inv in HeqR0.
-          destruct HeqR0 as [J1 J2]. auto.
-          left. simpl_env. fsetdec.
-      rewrite_env ((prefix ++ [(l0, l1)]) ++ acc) in H.
-      apply IHacc in H; simpl_env; simpl; auto.
-Qed.
-
-Lemma find_next_sub_predtree_wf_predtree: 
-  forall f idoms (Hwfi: WF_idoms f idoms) pdt (Hwf:WF_predtree f pdt) 
-    others pdt' others'
-  (Hdis: forall l0, 
-    In l0 others -> 
-    l0 `notin` dom pdt `union` cdom pdt),
-  find_next_sub_predtree idoms pdt others = ret (pdt', others') ->
-  WF_predtree f pdt'.
-Proof.
-  intros.
-  unfold find_next_sub_predtree in H.
-  change pdt with (nil++pdt) in H, Hdis at 1.
-  eapply find_next_sub_predtree_aux_wf_predtree in H; eauto.
-Qed.
-
-Lemma create_predtree_aux__WF_predtree_aux: forall n, 
-  P_create_predtree_aux__WF_predtree n.
-Proof.
-  intro n.
-  apply lt_wf_rec. clear n.
-  intros n IH.
-  unfold P_create_predtree_aux__WF_predtree in *.
-  intros f idoms Hwfi pdt0 others pdt Hdis Hlen Hwf.
-  destruct others as [|l1 others]; simple_create_predtree_aux.
-    intro J. inv J; auto.
-
-    remember (find_next_sub_predtree idoms pdt0 (l1 :: others)) as R.
-    destruct R as [[acc' others']|].
-      repeat fold_sub create_predtree_aux_func ; simpl proj1_sig.
-      fold (create_predtree_aux others' idoms acc').
-      intro J. subst.
-      apply IH with (m:=length others') (f:=f) in J; auto.
-        eapply find_next_sub_predtree_length; eauto.
-        eapply find_next_sub_predtree_fresh; eauto.
-        eapply find_next_sub_predtree_wf_predtree; eauto.
-      intro J. inv J.
-Qed.
-
-Lemma create_predtree_aux__WF_predtree : forall f idoms 
-  (Hwfi: WF_idoms f idoms) pdt0 others pdt
-  (Hdis: forall l0, 
-    In l0 others -> 
-    l0 `notin` dom pdt0 `union` cdom pdt0),
-  WF_predtree f pdt0 ->
-  create_predtree_aux others idoms pdt0 = Some pdt ->
-  WF_predtree f pdt.
-Proof.
-  intros.
-  assert (J:=@create_predtree_aux__WF_predtree_aux (List.length others)).
-  unfold P_create_predtree_aux__WF_predtree in J. eauto.
-Qed.
-
-Program Fixpoint create_dtree_aux (others:set l) (res: AMap.t (set l)) 
-  (root:l) {measure (List.length others)}
-  : option DTree :=
-match find_children res root others nil with
-| Some nil => Some (DT_node root DT_nil)
-| Some children =>
-    let others' := 
-      fold_left (fun acc l1 => List.remove id_dec l1 acc) children others in
-    let op_dts0 :=
-      (fold_left 
-        (fun acc l1 => 
-         match acc, create_dtree_aux others' res l1 with
-         | Some dts0, Some dt0 => Some (DT_cons dt0 dts0) 
-         | _, _ => None
-         end)
-        children (Some DT_nil)) in
-    match op_dts0 with
-    | Some dts0 => Some (DT_node root dts0)
-    | _ => None
-    end
-| _ => None 
-end.
-Next Obligation. 
-  symmetry in Heq_anonymous.
-  apply fold_left_remove_in_length; auto.
-    apply find_children_spec2 in Heq_anonymous; auto.
-    apply find_children_spec1 in Heq_anonymous; auto.
-    intro J. subst. auto.
-Qed.
-Next Obligation. split; intros; congruence. Qed.
-
-Lemma find_next_child__imm_domination: forall f idoms (Hwfi: WF_idoms f idoms) 
-  l1 others l2,
-  find_next_child idoms l1 others = ret l2 ->
-  imm_domination f l1 l2.
-Proof.
-  induction idoms; simpl; intros.
-    inv H.
-
-    destruct a.
-    inv Hwfi.
-    destruct (l_dec l0 l1); subst; eauto.
-      destruct (in_dec l_dec l3 others); eauto.
-        inv H. auto.
-Qed.
-
-Lemma init_predtree__WF_predtree : forall f root 
-  (Hentry:getEntryLabel f = Some root) idoms 
-  (Hwfi: WF_idoms f idoms) others pdt0 others0,
-  init_predtree idoms root others = Some (pdt0, others0) ->
-  WF_predtree f pdt0.
-Proof.
-  induction idoms; simpl; intros.
-    inv H.
-
-    destruct a.
-    inv Hwfi.
-    destruct (l_dec l0 root); subst; eauto.
-      destruct (in_dec l_dec l1 others); inv H.
-      apply WPDT_entry; auto.
-Qed.
-
-Lemma init_predtree__disjoint: forall root idoms others pdt0 others0,
-  init_predtree idoms root others = ret (pdt0, others0) ->
-  ~ In root others ->
-  forall l0 : atom, In l0 others0 -> l0 `notin` union (dom pdt0) (cdom pdt0).
-Proof.
-  induction idoms; simpl; intros.
-    inv H.
-
-    destruct a.
-    destruct (l_dec l1 root); subst.
-      destruct (in_dec l_dec l2 others); inv H.
-        simpl.
-        assert (l0 <> l2) as Hneq.
-          assert (J':=@remove_In _ l_dec others l2).
-          destruct (l_dec l0 l2); subst; auto.
-        assert (In l0 others) as Hin'.
-          apply remove_neq_in' in H1; auto.
-        assert (l0 <> root) as Hneq'.
-          destruct (l_dec l0 root); subst; auto.
-        fsetdec.
-
-      eapply IHidoms in H; eauto.        
-Qed.
-
-Lemma compute_idoms__WF_idoms_aux: forall f rd idoms acc,
-  reachablity_analysis f = Some rd ->
-  WF_idoms f acc ->
-  compute_idoms (dep_doms__nondep_doms (bound_fdef f) (dom_analyze f)) rd acc 
-    = idoms ->
-  WF_idoms f idoms.
-Proof.
-  induction rd; simpl; intros; subst; auto.
-    remember 
-      (find_idom (dep_doms__nondep_doms (bound_fdef f) (dom_analyze f)) a) as R.
-    destruct R.
-      apply IHrd with (acc:=(l0, a) :: acc); auto.
-        admit.
-        apply WF_idoms_cons; auto.
-          admit.
-      apply IHrd with (acc:=acc); auto.
-        admit.
-Qed.
-
-Lemma compute_idoms__WF_idoms: forall f rd idoms,
-  reachablity_analysis f = Some rd ->
-  compute_idoms (dep_doms__nondep_doms (bound_fdef f) (dom_analyze f)) rd nil 
-    = idoms ->
-  WF_idoms f idoms.
-Proof.
-  intros.
-  apply compute_idoms__WF_idoms_aux in H0; auto.
-    apply WF_idoms_nil.
-Qed.
-
-Lemma init_create_predtree_aux__WF_predtree : forall f idoms pdt0 others 
-  pdt root rd,
-  getEntryLabel f = Some root ->
-  reachablity_analysis f = Some rd ->
-  compute_idoms (dep_doms__nondep_doms (bound_fdef f) (dom_analyze f)) rd nil 
-    = idoms ->
-  init_predtree idoms root (List.remove eq_atom_dec root rd) 
-    = Some (pdt0, others) ->
-  create_predtree_aux others idoms pdt0 = Some pdt ->
-  WF_predtree f pdt.
-Proof.
-  intros.
-  eapply compute_idoms__WF_idoms in H1; eauto.
-  eapply create_predtree_aux__WF_predtree in H3; eauto.
-    eapply init_predtree__disjoint; eauto.
-      apply remove_In.
-    eapply init_predtree__WF_predtree; eauto.
-Qed.
-
-Scheme dtree_rec2 := Induction for DTree Sort Set
-  with dtrees_rec2 := Induction for DTrees Sort Set.
-
-Definition dtree_mutrec P P' :=
-  fun h1 h2 h3 => 
-    (pair (@dtree_rec2 P P' h1 h2 h3) (@dtrees_rec2 P P' h1 h2 h3)).
-
-Definition dtree_insert__wf_dtree_prop (dt1:DTree) := 
-forall f a1 a0 dt2,
-  WF_dtree f dt1 ->
-  dtree_insert dt1 a1 a0 = ret dt2 ->
-  WF_dtree f dt2.
-
-Definition dtrees_insert__wf_dtrees_prop (dts1:DTrees) := 
-forall f root a1 a0 dts2,
-  WF_dtrees f root dts1 ->
-  dtrees_insert dts1 a1 a0 = ret dts2 ->
-  WF_dtrees f root dts2.
-
-Lemma dtree_insert__wf_dtree_mutrec :
-  (forall dt1, dtree_insert__wf_dtree_prop dt1) *
-  (forall dts1, dtrees_insert__wf_dtrees_prop dts1).
-Proof.
-  apply dtree_mutrec; 
-    unfold dtree_insert__wf_dtree_prop, dtrees_insert__wf_dtrees_prop;
-    simpl; intros.
-
-    inv H0.
-    destruct (id_dec a1 l0); subst.
-      inv H1.
-      apply WDT_node; simpl; auto.
-        admit.
-        apply WDT_cons; simpl; auto.
-          admit.
-          admit.
-          apply WDT_node; simpl; auto.
-            admit.
-            apply WDT_nil.
-       
-      remember (dtrees_insert d a1 a0) as R.
-      destruct R; inv H1. 
-        apply WDT_node; simpl; eauto.
-          admit.
-        
-    inv H0. auto.
-
-    remember (dtree_insert d a1 a0) as R.
-    destruct R; inv H2. 
-    remember (dtrees_insert d0 a1 a0) as R.
-    destruct R; inv H4. 
-    inv H1.
-    apply WDT_cons; simpl; eauto.
-      admit.
-      admit.
-Qed.
-
-Lemma dtree_insert__wf_dtree: forall f a1 a0 dt1 dt2,
-  WF_dtree f dt1 ->
-  dtree_insert dt1 a1 a0 = ret dt2 ->
-  WF_dtree f dt2.
-Proof.
-  induction dt1; simpl; intros.
-    destruct (id_dec a1 l0); subst.
-      inv H0.
-      inv H.
-      apply WDT_node; simpl; auto.
-        admit.
-        apply WDT_cons; simpl; auto.
-          admit.
-          admit.
-          apply WDT_node; simpl; auto.
-            admit.
-            apply WDT_nil.
-       
-      remember (dtrees_insert d a1 a0) as R.
-      destruct R.
-        inv H0. auto.
-
-
-Admitted.
-
-Lemma tree2dtree__wf_dtree: forall f vs es tree dt,
-  tree2dtree vs es tree = Some dt -> WF_dtree f dt.
-Proof.
-  induction tree; simpl; intros.
-    destruct r. inv H.
-    apply WDT_node.
-      admit.
-      simpl. fsetdec.
-      apply WDT_nil.
-
-    destruct f0. destruct n.
-    remember (tree2dtree v a tree) as R.
-    destruct R.
-      eapply dtree_insert__wf_dtree in H; eauto.
-      inv H.
-
-    apply IHtree in H; auto.
-Qed.
-*)
-
-(*
-Definition create_dtree (f: fdef) : option DTree :=
-match getEntryBlock f, reachablity_analysis f with
-| Some (block_intro root _ _ _), Some rd =>
-    let 'dt := dom_analyze f in
-    let 'b := bound_fdef f in
-    create_dtree_aux (dep_doms__nondep_doms b dt) root 
-      (List.remove eq_atom_dec root rd)
-| _, _ => None
-end.
-*)
 
 (*****************************)
 (*
